ironfleet/src/Dafny/Distributed/Concur/UltimateReduction.i.dfy
@@ -16,9 +16,15 @@ module UltimateReductionModule {
         )
         requires IsValidSystemTraceAndBehavior(config, trace, lb);
         requires IsValidReductionPlan(config, plan);
+        requires forall entry :: entry in trace ==> IsRealAction(entry.action);
         requires forall actor :: actor in config.tracked_actors ==>
                      RestrictTraceToTrackedActions(RestrictTraceToActor(trace, actor)) == GetEntries(plan[actor].trees);
         ensures  SystemBehaviorRefinesSpec(lb);
+    {
+        var mb := lemma_RefineToBehaviorWithoutStates(config, trace, lb);
+        lemma_ReductionOfBehaviorWithoutStates(config, trace, mb, plan);
+        lemma_SystemSpecRefinementConvolutionExtraPure(lb, mb);
+    }
 
 }
 
